hax-lib/proof-libs/lean/Hax/test/HaxMvcgenAt.lean
@@ -1,0 +1,37 @@
+import Hax
+
+open Std.Do
+
+-- A custom operation with no spec in any specset
+def myOp (a b : u64) : RustM u64 := pure (a + b)
+
+-- Example with an operation without spec
+-- set_option hax_mvcgen.specset "int" in
+-- example (a b : u64) (h : ⦃ ⌜ True ⌝ ⦄ (do (← myOp a b) >? 0) ⦃ ⇓r => ⌜ r ⌝ ⦄) : True := by
+--   hax_mvcgen at h
+--   sorry
+
+
+@[specset int]
+theorem haxAdd_spec {x y : u64} :
+    ⦃ ⌜ True ⌝ ⦄ (x +? y) ⦃ ⇓? r => ⌜ r.toNat = x.toNat + y.toNat ⌝ ⦄ := by sorry
+
+
+
+set_option hax_mvcgen.specset "int" in
+example (a b : u64) (h : ⦃ ⌜ True ⌝ ⦄ (do (← a +? b) >? 0) ⦃ ⇓r => ⌜ r ⌝ ⦄) : True := by
+  hax_mvcgen at h
+  apply True.intro
+
+
+set_option hax_mvcgen.specset "int" in
+example (a b : u64) (h : ∀ i, ⦃ ⌜ True ⌝ ⦄ (do (← a +? b) >? i) ⦃ ⇓r => ⌜ r ⌝ ⦄) :  a + b > 0 := by
+  hax_mvcgen at h
+  apply h
+  grind
+  sorry
+
+set_option hax_mvcgen.specset "int" in
+example (a b : u64) (h : ⦃ ⌜ True ⌝ ⦄ (do if ← (← a +? b) >? 0 then pure true else pure false) ⦃ ⇓r => ⌜ r ⌝ ⦄) : True := by
+  hax_mvcgen at h
+  apply True.intro
